\documentclass{article}
\usepackage{fancyhdr}
\pagestyle{fancy}
\fancyfoot{}
\fancyfoot[C]{\thepage}
\rhead{Yarosevich - 1064712}
\usepackage{setspace}
\usepackage{siunitx} % Provides the \SI{}{} and \si{} command for typesetting SI units
\usepackage{graphicx} % Required for the inclusion of images
\usepackage{amsmath} % Required for some math elements 
\usepackage[export]{adjustbox} % loads also graphicx
\usepackage{listings}
\usepackage{setspace}
\usepackage{matlab-prettifier}
\usepackage{physics}
\usepackage{float}
\usepackage[most]{tcolorbox}
\usepackage{amsfonts}
\usepackage{color}
\usepackage{titlesec}
\usepackage{caption}
\usepackage{subcaption}
\usepackage{placeins}
\usepackage{bm}
\usepackage{esvect}
\newcommand{\uveci}{{\bm{\hat{\textnormal{\bfseries\i}}}}}
\newcommand{\uvecj}{{\bm{\hat{\textnormal{\bfseries\j}}}}}
\DeclareRobustCommand{\uvec}[1]{{%
  \ifcsname uvec#1\endcsname
     \csname uvec#1\endcsname
   \else
    \bm{\hat{\mathbf{#1}}}%
   \fi
}}


\newcommand{\R}{\mathbb{R}}

\usepackage{xcolor}

\DeclareCaptionFont{white}{\color{white}}
\DeclareCaptionFormat{listing}{%
  \parbox{\textwidth}{\colorbox{gray}{\parbox{\textwidth}{#1#2#3}}\vskip-4pt}}
\captionsetup[lstlisting]{format=listing,labelfont=white,textfont=white}
\lstset{frame=lrb,xleftmargin=\fboxsep,xrightmargin=-\fboxsep}
\titleformat{\section}[runin]
  {\normalfont\Large\bfseries}{\thesection}{1em}{}
\titleformat{\subsection}[runin]
  {\normalfont\large\bfseries}{\thesubsection}{1em}{}


\setlength\parindent{0pt} % Removes all indentation from paragraphs

\renewcommand{\labelenumi}{\alph{enumi}.} % Make numbering in the enumerate environment by letter rather than number (e.g. section 6)

%\usepackage{times} % Uncomment to use the Times New Roman font

%----------------------------------------------------------------------------------------
%	DOCUMENT INFORMATION
%----------------------------------------------------------------------------------------

\title{AMATH 503: Homework 5 \\Due May, 28 2019 \\ ID: 1064712} % Title

\author{Trent \textsc{Yarosevich}} % Author name

\date{\today} % Date for the report

\begin{document}
\maketitle % Insert the title, author and date
\setlength\parindent{1cm}

\begin{center}
\begin{tabular}{l r}
%Date Performed: December 1, 2017 \\ % Date the experiment was performed
Instructor: Professor Ka-Kit Tung % Instructor/supervisor
\end{tabular}
\end{center}
\doublespacing
% If you wish to include an abstract, uncomment the lines below
% \begin{abstract}
% Abstract text
% \end{abstract}

%----------------------------------------------------------------------------------------
%	SECTION 1
%----------------------------------------------------------------------------------------
\section*{\textbf{(1)}}
If we use the eigenfunction and eigenvalue from the prompt, assuming we started with a a $\lambda^2$ in the function and not $\lambda$, we have:
\begin{equation}
\begin{aligned}
\phi_p = J_p(\lambda r)\\
\lambda_{pj} = \frac{z_{jp}}{a}\\
\end{aligned}
\end{equation}
Where $z_{jp}$ is the $p$'th zero of $J$. We know from the notes that for a cylindrical Bessel's function like this, we have the following values for $p,r,q$ when $b=0$ as it does here. 
\begin{equation}
\begin{aligned}
p(r) = \lambda r\\
r(r) = \lambda r\\
q(r) = \frac{p^2}{\lambda r}\\
\end{aligned}
\end{equation}
We now consider two pairs of eigenfunctions and eigenvalues:
\begin{equation}
\begin{aligned}
\phi_k = J_k(\lambda r); \lambda_k =\frac{z_{pk}}{a}\\ \\
\phi_j = J_j(\lambda r); \lambda_j =\frac{z_{pj}}{a}\\ \\
\end{aligned}
\end{equation}
Plugging these into the Bessel function:
\begin{equation}
\begin{aligned}
(p\phi_k')' + (\lambda_k x - \frac{p^2}{x})\phi_k = 0\\
(p\phi_j')' + (\lambda_j x - \frac{p^2}{x})\phi_j = 0\\
\end{aligned}
\end{equation}
We then follow the logic of the general proof of S-L orthogonality by multiplying the first by $\phi_j$ and the second by $\phi_k$ then subtracting one from the other:
\begin{equation}
\begin{aligned}
\phi_j(p\phi_k')' - \phi_k(p\phi_j)' = (\lambda_j - \lambda_k)r\phi_j\phi_k
\end{aligned}
\end{equation}
The LHS is a derivative, so we rewrite as follows:
\begin{equation}
\begin{aligned}
\frac{d}{dr} \Big{[}\phi_j(p\phi_k')' - \phi_k(p\phi_j') \Big{]} = (\lambda_j - \lambda_k)r(r)\phi_j\phi_k\\
\end{aligned}
\end{equation}
We then integrate both sides giving:
\begin{equation}
\begin{aligned}
\Big{[}\phi_j(p\phi_k')' - \phi_k(p\phi_j') \Big{]}\Big{|}_0^a = (\lambda_j - \lambda_k)\int_0^ar(r)\phi_j\phi_kdr\\
\end{aligned}
\end{equation}
We can observe here that the LHS goes to zero because (i) p(0) = 0, and (ii) because at the boundary $a$ the eigenfunctions will be $\phi_{j/k} = J_{j/k}(z_{mn}(\frac{a}{a})$ which goes to zero because the $a$'s cancel, leaving only the zero of the eigenfunction. This results in:
\begin{equation}
 \begin{aligned}
 (\lambda_j - \lambda_k)\int_0^ar(r)\phi_j\phi_kdr = 0
\end{aligned}
\end{equation}
We can now simply observe that, if $\lambda_j = \lambda_k$, the leading constant becomes zero, and the integral becomes:
\begin{equation}
\begin{aligned}
\int_0^ar(r)(\phi_j)^2dr
\end{aligned}
\end{equation}
This integral is a positive constant since the Bessel function defines $r(r)>0$, and the eigenfunction is squared.
\\
Alternatively, if $\lambda_j \neq \lambda_k$, this integral must be identically zero. The resulting integral is thus:
\begin{tcolorbox}[minipage,colback=white,arc=0pt,outer arc=0pt]
\begin{equation}
\begin{aligned}
\int_0^ar(r)\phi_k\phi_j dr =
 \begin{cases} 
      0, & \lambda_k \neq \lambda_j \\
      c, & \lambda_k = \lambda_j
   \end{cases}
\end{aligned}
\end{equation}
Where $c>0$ is a constant.
\end{tcolorbox}
\section*{\textbf{(2)}}
\subsection*{\textbf{(a)}}
It is extremely unclear to me what this problem is asking, and so I'm going to follow the derivation of the D'Alembert solution in the context of the problem.\\
\\
From the prompt we know that, with spherical symmetry, the 3D wave equation becomes:
\begin{equation}
\begin{aligned}
u_{tt} = \frac{c^2}{r}(ru)_{rr}
\end{aligned}
\end{equation}
Bringing the $r$ to the LHS, we can note that it is constant variable with respect to $t$, and we can write the PDE as:
\begin{equation}
\begin{aligned}
(ru)_{tt} = c^2(ru)_{rr}
\end{aligned}
\end{equation}
Let $z = ru$, and then we proceed to a D'Alembert solution, starting with a variable transform:
\begin{equation}
\begin{aligned}
k = r+ct, s = r-ct\\
r= \frac{1}{2}(r+s), t = \frac{1}{2c}(r - s)\\
\end{aligned}
\end{equation}
The differential operators are now:
\begin{equation}
\begin{aligned}
\pdv{}{r} = \pdv{}{t}\pdv{t}{k} + \pdv{}{r}\pdv{r}{k} = \frac{1}{2c}\pdv{}{t} + \frac{1}{2}\pdv{}{r} = \frac{1}{2c}(\pdv{}{t} + c\pdv{}{r})\\
\pdv{}{s} = \pdv{}{t}\pdv{t}{s} + \pdv{}{r}\pdv{r}{s} = -\frac{1}{2c}\pdv{}{t} + \frac{1}{2}\pdv{}{r} = -\frac{1}{2c}(\pdv{}{t} + c\pdv{}{r})\\
\end{aligned}
\end{equation}
Now if:
\begin{equation}
\begin{aligned}
\pdv[2]{}{t}z -c^2\pdv[2]{}{r}z = 0\\
(\pdv[2]{}{t} - c^2 \pdv[2]{}{r})z = 0\\
(\pdv{}{t} - c^2 \pdv{}{r})(\pdv{}{t} - c^2 \pdv{}{r})z = 0\\
\text{using our differential operators above:}\\
(2c \pdv{}{k})(-2c\pdv{}{s})z = 0\\
(-4c^2)\pdv{}{k}\pdv{}{s}z = 0\\
\pdv{}{k}\pdv{}{s}z = 0\\
\end{aligned}
\end{equation}
Solving this we get:
\begin{equation}
\begin{aligned}
\pdv{z}{s} = f(s)\\
\text{where $f(s)$ is some function of $s$.}\\
z(s,k) = \int f(s) + G(k)\\
\text{where $G(k)$ is some function of $k$.}\\
z(s,k) = F(s) + G(k)\\
\text{Where $F$ is the antiderivative of $f$:}\\
\end{aligned}
\end{equation}
Substituting the original functions of $k/s$:
\begin{equation}
\begin{aligned}
z(r,t) = F(r-ct) + G(r+ct)\\
\end{aligned}
\end{equation}
Fitting this to general initial conditions:
\begin{equation}
\begin{aligned}
z(r,0) = F(r) + G(r) = z_0
z_t(r,t) = -cF'(r - ct) + cG'(r-ct)\\
z_t(r,0) = -cF'(r) + cG'(r) = v_0
\end{aligned}
\end{equation}
Integrating in order to get two equations with the same form of $F$ and $G$:
\begin{equation}
\begin{aligned}
-cF(r) + cG(r) = \int_0^r v_0(\bar{x})d\bar{x}
\end{aligned}
\end{equation}
Now we multiply $z(r,0)$ above by $c$ and add it to the second equation:
\begin{equation}
\begin{aligned}
2cG(r) = \int_0^r v_0(\bar{x})d\bar{x} + cz_0(r)\\
G(x) = \frac{1}{2c}(\int_0^r v_0(\bar{x})d\bar{x}) + \frac{1}{2}z_0(r)\\
\end{aligned}
\end{equation}
Next we multiply $z(r,0)$ by $-c$ and add to the second equation:
\begin{equation}
\begin{aligned}
-2cF(r) = -c z_0(r)  +  \int_0^r v_0(\bar{x})d\bar{x}\\
F(r) = \frac{1}{2}z_0(r) - \frac{1}{2c}(\int_0^r v_0(\bar{x})d\bar{x}) 
\end{aligned}
\end{equation}
To get our solution we simply plug these into our original function above, and combine the integrals by changing the sign of the second one and swapping its bounds of integration.
\begin{equation}
\begin{aligned}
z(r,t) = \frac{1}{2}(z_0(r-ct) + z_0(r + ct)) + \frac{1}{2c}\int_{r-ct}^{r+ct}v_0(\bar{x})d\bar{x}
\end{aligned}
\end{equation}
Allowing that $u = \frac{z}{r}$ the final solution is:
\begin{tcolorbox}[minipage,colback=white,arc=0pt,outer arc=0pt]
\begin{equation}
\begin{aligned}
u(r,t) = \frac{1}{2r}(z_0(r-ct) + z_0(r + ct)) + \frac{1}{2rc}\int_{r-ct}^{r+ct}v_0(\bar{x})d\bar{x}
\end{aligned}
\end{equation}
\end{tcolorbox}
\subsection*{\textbf{(b)}}
The outgoing wave is the one determined by $z_0(r-ct)$, since this is the compression wave corresponding with an increasing $r$ as $t$ increases in order to track the wave's movement.


% Now let's substitute $v= ru$ and plug the resulting equation into the D'Alembert Solution:
% \begin{equation}
% \begin{aligned}
% v_{tt} = c^2v_{rr}\\
% v(r,t) = \frac{1}{2} \Big{[}g(r - ct) + g(r + ct) + \frac{1}{2c}\int^{r+ct}_{r-ct}h(s)ds
% \end{aligned}
% \end{equation}
% To transform $g$ back to its equivalent term in $u$:
% \begin{equation}
% \begin{aligned}
% v(r,0) = g(r)\\
% \end{aligned}
% \end{equation}
% And the final form of the equation is:
% \begin{equation}
% \begin{aligned}
% u(r,0) = f(r)
% \end{aligned}
% \end{equation}
% Thus we have:
% \begin{equation}
% \begin{aligned}
% \frac{1}{r}v(r,0) = u(r,0)\\
% \frac{1}{r}g(r) = f(r)\\
% g(r) = r f(r)\\
% \end{aligned}
% \end{equation}
% Similarly, we observe that:
% \begin{equation}
% \begin{aligned}
% v_t = \frac{d}{dt} \Big{[}\frac{1}{2c}\int^{r+ct}_{r-ct}h(s)ds \Big{]}\\
% v_t =\frac{1}{2c} \frac{d}{dt} \Big{[}H(r+ct) - H(r-ct) \Big{]}\\
% v_t = \frac{1}{2c} \Big{[}h(r+ct)(c) - h(r-ct)(-c)\Big{]}\\
% v_t = \frac{1}{2} \Big{[}h(r+ct) + h(r-ct)\\
% v_t(r,0) = h(r)\\
% ru_t(r,0) = h(r)\\
% u_t(r,0) = \frac{1}{r}h(r)\\
% \text{So we define some new function:}\\
% u_t(r,0) = k(r)\\
% rk(r) = h(r)
% \end{aligned}
% \end{equation}
% We then substitute all the transformed terms into the solution and replace the $r$ terms with suitable $r\pm ct$ or $s$ and get:
% \begin{tcolorbox}[minipage,colback=white,arc=0pt,outer arc=0pt]
% \begin{equation}
% \begin{aligned}
% ru(r,t) = \frac{1}{2} \Big{[}(r-ct)f(r-ct) + (r+ct)f(r+ct) + \frac{1}{2c}\int_{r-ct}^{r+ct}sk(s)ds\\
% u(r,t) = \frac{1}{2r} \Big{[}(r-ct)f(r-ct) + (r+ct)f(r+ct) + \frac{1}{2c}\int_{r-ct}^{r+ct}sk(s)ds\\
% \end{aligned}
% \end{equation}
% \end{tcolorbox}
\section*{\textbf{(3)}}
\subsection*{\textbf{(a)}}
In the steady state solution $u_{tt} = 0$ thus:
\begin{equation}
\begin{aligned}
u_{xx} = - 1\\
u_x = -x + c\\
u = \frac{-x^2}{2} + cx + d\\
u(0)= 0 = d\\
u(1) = 0 = -\frac{1}{2} + c\\
c = \frac{1}{2}
\end{aligned}
\end{equation}
So the steady state solution is:
\begin{tcolorbox}[minipage,colback=white,arc=0pt,outer arc=0pt]
\begin{equation}
\begin{aligned}
u(x,t)  = \frac{-x^2}{2} + \frac{x}{2}
\end{aligned}
\end{equation}
\end{tcolorbox}
Suppose the transient solution is some $v = u - u_{\text{steady}}$. If we plug this into the PDE we get:
\begin{equation}
\begin{aligned}
v_{tt} - 0 = v_{xx} - \frac{d^2}{dx^2}(\frac{-x^2}{2} + \frac{x}{2}) + 1\\
v_{tt} = v_{xx}
\end{aligned}
\end{equation}
By separation of variables let $v=T(t)X(x)$. As we've seen countless times in the class thus far, this yields the solution:
\begin{equation}
\begin{aligned}
v(x,t) = \sum_{n=1}^{\infty} \Big{[}A_nsin(\lambda_n t) + B_ncos(\lambda_n t) \Big{]}sin(\frac{n\pi x}{L})\\
L = 1\\
\end{aligned}
\end{equation}
Now we apply the BCs noting that $u(x,t) = v(x,t) - \frac{x^2}{2} + \frac{x}{2}$\\
\begin{equation}
\begin{aligned}
u(x,0) = 0 = \sum_{n=1}^{\infty}B_nsin(n\pi x)- \frac{x^2}{2} + \frac{x}{2}\\
\sum_{n=1}^{\infty}B_nsin(n\pi x) = \frac{x^2}{2} - \frac{x}{2}\\
\end{aligned}
\end{equation}
This is a sine series and the coefficient $B_n$ s given:
\begin{equation}
\begin{aligned}
B_n = \int_0^1x^2sin(n\pi x)dx - \int_0^1xsin(n\pi x)dx\\
\end{aligned}
\end{equation}
Proceeding one integral at a time:
\begin{equation}
\begin{aligned}
\int_0^1x^2sin(n\pi x)dx = \Big{[}\frac{-x^2cos(n\pi x)}{n\pi} \Big{]}\Big{|}_0^1 + 2\int_0^1\frac{xcos(n\pi x)}{n\pi}dx\\
\int_0^1\frac{xcos(n\pi x)}{n\pi}dx = \Big{[}\frac{xsin}{(n^2\pi^2} \Big{]}\Big{|}_0^1 - \int_0^1\frac{sin(n\pi x)}{n^2\pi^2}dx\\
\int_0^1\frac{sin(n\pi x)}{n^2\pi^2}dx = \Big{[}\frac{cos(n\pi x)}{n^3\pi^3}\Big{]}\Big{|}_0^1
\end{aligned}
\end{equation}
Putting these evaluations together we have:
\begin{equation}
\begin{aligned}
 \Big{[}\frac{-x^2cos(n\pi x)}{n\pi} \Big{]}\Big{|}_0^1 & + 2 \Big{[}\Big{[}\frac{xsin}{(n^2\pi^2} \Big{]}\Big{|}_0^1 + \Big{[}\frac{cos(n\pi x)}{n^3\pi^3}\Big{]}\Big{|}_0^1 \Big{]}\\
 &= \frac{-(-1)^n}{n\pi} + 2 \Big{[}\frac{(-1)^n)}{n^3\pi^3} - \frac{1}{n^3\pi^3} \Big{]}
\end{aligned}
\end{equation}
Now the other integral:
\begin{equation}
\begin{aligned}
\int_0^1xsin(n\pi x)dx = \Big{[}\frac{-x cos(n\pi x)}{n\pi} \Big{]}\Big{|}_0^1 - \int_0^1\frac{cos(n\pi x)}{n\pi}dx\\
\int_0^1\frac{cos(n\pi x)}{n\pi}dx = \Big{[} \frac{sin(n\pi x)}{n^2\pi^2} \Big{]} \Big{|}_0^1 = 0\\
\int_0^1xsin(n\pi x)dx = \frac{-(-1)^n}{n\pi}
\end{aligned}
\end{equation}
Combining the two terms:
\begin{equation}
\begin{aligned}
B_n = \frac{-(-1)^n n^2\pi^2 + 2(-1)^n - 2 + (-1)^nn^2\pi^2}{n^3\pi^3}\\
B_n = \frac{2( (-1)^n - 1)}{n^3\pi^3}
\end{aligned}
\end{equation}
Now we define $n = 1,3,5...$ giving:
\begin{equation}
\begin{aligned}
B_n = \frac{-4}{n^3\pi^3}
\end{aligned}
\end{equation}
Applying the other initial condition we take the derivative:
\begin{equation}
\begin{aligned}
u_t(x,t) = \sum_{n=1}^{\infty} \Big{[}n\pi  A_ncos(n\pi t) - n\pi B_nsin(n\pi t) \Big{]}sin(n\pi x)\\
u_t(x,0) = \sum_{n=1}^{\infty}n\pi A_n sin(n\pi x) = 0\\
A_n = 0
\end{aligned}
\end{equation}
Thus the transient solution and complete solution are:
\begin{tcolorbox}[minipage,colback=white,arc=0pt,outer arc=0pt]
\begin{equation}
\begin{aligned}
v(x,t) = \sum_{n=1}^{\infty}\frac{-4}{n^3\pi^3}cos(n\pi t)sin(n\pi x)\\
u(x,t) = \sum_{n=1}^{\infty}\frac{-4}{n^3\pi^3}cos(n\pi t)sin(n\pi x) - \frac{x^2}{2} + \frac{x}{2}\\
n = 1,3,5...
\end{aligned}
\end{equation}
\end{tcolorbox}
\subsection*{\textbf{(b)}}
First we determine the eigenfunctions and eigenvalues that will satisfy the boundary conditions. They are homogeneous dirchelet, and so the eigenfunction is $sin(n\pi x)$. We thus represent the homogeneous form of the PDE as:
\begin{equation}
\begin{aligned}
u(x,t) = \sum_{n=1}^{\infty}T(t)sin(n\pi x)
\end{aligned}
\end{equation}
We then represent the forcing term with the eigenfunction/values:
\begin{equation}
\begin{aligned}
f(x,t) = 1 = \sum_{n=1}^{\infty}f_n sin(n\pi x)
\end{aligned}
\end{equation}
Next we plug this into the PDE. 
\begin{equation}
\begin{aligned}
\sum_{n=1}^{\infty} T_n''(t)X(x) - X_n''(x)T_n(t) = \sum_{n=1}^{\infty}f_n sin(n\pi x)\\
T_n''(t)sin(n\pi x) + (n\pi)^2 sin(n\pi x)T_n(t) = f_nsin(n\pi x)\\
T_n''(t) + (n\pi)^2T_n(t) = f_n
\end{aligned}
\end{equation}
To proceed we'll need $f_n$, which is the coefficient for the sine series for $f(x) = 1$:
\begin{equation}
\begin{aligned}
A_n  = 2\int_0^1sin(n\pi x) = 2\Big{[}\frac{-cos(n\pi x)}{n\pi}\Big{]}\Big{|}_0^1\\
A_n = 2\frac{1-(-1)^n}{n\pi}\\
A_n = 0 \text{ for even } n,\\
A_n = \frac{4}{n\pi} \text{ for odd } n
\end{aligned}
\end{equation}
We thus have two scenarios:
\begin{equation}
\begin{aligned}
n = 1, 3, 5... &\to T_n''(t) + (n\pi)^2T_n(t) = \frac{4}{n\pi}\\
n = 2, 4, 6... &\to T_n''(t) + (n\pi)^2T_n(t) = 0
\end{aligned}
\end{equation}
In the even case, we know from major precedent that the solution is sines and cosines:
\begin{equation}
\begin{aligned}
n = 2,4,6...\\
T_n(t) = A_n sin(n\pi t) + B_n cos(n\pi t)
\end{aligned}
\end{equation}
For the odd $n$ case we need the homogeneous solution plus the particular. We already have the former, and so to find the particular solution we guess a solution in the form of the forcing term, i.e. a constant $k$ and plug it into the PDE:
\begin{equation}
\begin{aligned}
T(t)_{\text{particular}} = k\\
k(n\pi)^2= \frac{4}{n\pi}\\
k = \frac{4}{(n\pi)^3}
\end{aligned}
\end{equation}
Thus the complete solution for $T(t)$ for odd $n$ is:
\begin{equation}
\begin{aligned}
T_n(t) = \sum_{n=1}^{\infty}A_n sin(n\pi t) + B_n cos(n\pi t) + \frac{4}{(n\pi)^3}
\end{aligned}
\end{equation}
Now, I'm not sure how to articulate this accurately, but I think the $n=2,4,6..$ case is not a part of the solution, since it actually doesn't satisfy the PDE. I speculate that this is because $f_n$ can be defined with strictly odd $n$. We will need to solve the homogeneous case, but the general solution is of the form:
\begin{tcolorbox}[minipage,colback=white,arc=0pt,outer arc=0pt]
\begin{equation}
\begin{aligned}
u(x,t) = \sum_{n=1}^{\infty} \Big{[} A_n sin(n\pi t) + B_n cos(n\pi t) +\frac{4}{(n\pi)^3} \Big{]}sin(n\pi x)\\
n = 1,3,5...
\end{aligned}
\end{equation}
\end{tcolorbox}

Applying the Initial Conditions:
\begin{equation}
\begin{aligned}
u(x,0) = \sum_{n=1}^{\infty} \Big{[}B_n + \frac{4}{(n\pi)^3}\Big{]}sin(n\pi x) = 0\\
B_n = -\frac{4}{(n\pi)^3}\\
u_t(x,t) = \sum_{n=1}^{\infty} \Big{[} n\pi A_n cos(n\pi t) - n\pi B_n sin(n\pi t) \Big{]}sin(n\pi x)\\
u_t(x,0) = \sum_{n=1}^{\infty}\Big{[}n\pi A_n \Big{]}sin(n\pi x) = 0\\
A_n = 0
\end{aligned}
\end{equation}
This gives a final solution of:
\begin{tcolorbox}[minipage,colback=white,arc=0pt,outer arc=0pt]
\begin{equation}
\begin{aligned}
u(x,t) = \sum_{n=1}^{\infty} \Big{[} \frac{4}{(n\pi)^3}( 1- cos(n\pi t)) \Big{]}sin(n\pi x)\\
n = 1,3,5...
\end{aligned}
\end{equation}
\end{tcolorbox}
If we note from \textbf{(22)} above that 
\begin{equation}
\begin{aligned}
n = 1,3,5..\\
\sum_{n=1}^{\infty}\frac{-4}{(n\pi)^3}sin(n\pi x) = \frac{x^2}{2} - \frac{x}{2}\\
\sum_{n=1}^{\infty}\frac{4}{(n\pi)^3}sin(n\pi x) = -\frac{x^2}{2} +\frac{x}{2}\\
\end{aligned}
\end{equation}
We can see that the extra series term in \textbf{(42)} is equivalent to the non-series term in \textbf{(30)} and we have the same answer.
\end{document}